\documentclass{article}
\usepackage{amsmath}
\usepackage{fouriernc}
\usepackage[a5paper]{geometry}

\DeclareMathOperator{\sgn}{sgn}
\DeclareMathOperator{\asin}{asin}
\DeclareMathOperator{\acos}{acos}
\DeclareMathOperator{\atan}{atan}
\DeclareMathOperator{\acot}{acot}
\DeclareMathOperator{\asec}{asec}
\DeclareMathOperator{\acsc}{acsc}
\DeclareMathOperator{\sech}{sech}
\DeclareMathOperator{\csch}{csch}
\DeclareMathOperator{\asinh}{asinh}
\DeclareMathOperator{\acosh}{acosh}
\DeclareMathOperator{\atanh}{atanh}
\DeclareMathOperator{\acoth}{acoth}
\DeclareMathOperator{\asech}{asech}
\DeclareMathOperator{\acsch}{acsch}

\begin{document}
    \begin{equation}
        c'=0
    \end{equation}
    \begin{equation}
        x'=1
    \end{equation}
    \begin{equation}
        (f(g(x)))'=f'(g(x))g'(x)
    \end{equation}
    \begin{equation}
        (f(x)+g(x))'=f'(x)+g'(x)
    \end{equation}
    \begin{equation}
        (f(x)-g(x))'=f'(x)-g'(x)
    \end{equation}
    \begin{equation}
        (f(x)g(x))'=f'(x)g(x)+f(x)g'(x)
    \end{equation}
    \begin{equation}
        \left(\frac{f(x)}{g(x)}\right)'=\frac{f'(x)g(x)-f(x)g'(x)}{g(x)^2}
    \end{equation}
    \begin{equation}
        \left(f(x)^c\right)'=cf(x)^{c-1}f'(x)
    \end{equation}
    \begin{equation}
        \left(c^{g(x)}\right)'=c^{g(x)}\ln(c)g'(x)
    \end{equation}
    \begin{equation}
        \left(f(x)^{g(x)}\right)'=f(x)^{g(x)}\left(\frac{f'(x)g(x)}{f(x)}+g'(x)\ln(f(x))\right)
    \end{equation}
    \begin{equation}
        \sgn'(x)=0
    \end{equation}
    \begin{equation}
        (|x|)'=\sgn(x)
    \end{equation}
    \begin{equation}
        (\sqrt{x})'=\frac{1}{2\sqrt{x}}
    \end{equation}
    \begin{equation}
        \exp'(x)=\exp(x)
    \end{equation}
    \begin{equation}
        \ln'(x)=\frac{1}{x}
    \end{equation}
    \begin{equation}
        \sin'(x)=\cos(x)
    \end{equation}
    \begin{equation}
        \cos'(x)=-\sin(x)
    \end{equation}
    \begin{equation}
        \tan'(x)=\sec(x)^2
    \end{equation}
    \begin{equation}
        \cot'(x)=-\csc(x)^2
    \end{equation}
    \begin{equation}
        \sec'(x)=\sec(x)\tan(x)
    \end{equation}
    \begin{equation}
        \csc'(x)=-\csc(x)\cot(x)
    \end{equation}
    \begin{equation}
        \asin'(x)=\sec(\asin(x))
    \end{equation}
    \begin{equation}
        \acos'(x)=-\csc(\acos(x))
    \end{equation}
    \begin{equation}
        \atan'(x)=\cos(\atan(x))^2
    \end{equation}
    \begin{equation}
        \acot'(x)=-\sin(\acot(x))^2
    \end{equation}
    \begin{equation}
        \asec'(x)=\cos(\asec(x))\cot(\asec(x))
    \end{equation}
    \begin{equation}
        \acsc'(x)=-\sin(\acsc(x))\tan(\acsc(x))
    \end{equation}
    \begin{equation}
        \sinh'(x)=\cosh(x)
    \end{equation}
    \begin{equation}
        \cosh'(x)=\sinh(x)
    \end{equation}
    \begin{equation}
        \tanh'(x)=\sech(x)^2
    \end{equation}
    \begin{equation}
        \coth'(x)=-\csch(x)^2
    \end{equation}
    \begin{equation}
        \sech'(x)=-\sech(x)\tanh(x)
    \end{equation}
    \begin{equation}
        \csch'(x)=-\csch(x)\coth(x)
    \end{equation}
    \begin{equation}
        \asinh'(x)=\sech(\asinh(x))
    \end{equation}
    \begin{equation}
        \acosh'(x)=\csch(\acosh(x))
    \end{equation}
    \begin{equation}
        \atanh'(x)=\cosh(\atanh(x))^2
    \end{equation}
    \begin{equation}
        \acoth'(x)=-\sinh(\acoth(x))^2
    \end{equation}
    \begin{equation}
        \asech'(x)=-\cosh(\asech(x))\coth(\asech(x))
    \end{equation}
    \begin{equation}
        \acsch'(x)=-\sinh(\acsch(x))\tanh(\acsch(x))
    \end{equation}
\end{document}